Iris/Iris/Algebra/Lib/MonoNat.lean
@@ -189,14 +189,14 @@ theorem auth_unpersist (n : MaxNat) :
 
 @[rocq_alias mono_nat_auth_dfrac_is_op]
 instance {dq dq1 dq2 : DFrac} {n : MaxNat}
-    [h : IsOp io dq dq1 dq2] :
-    IsOp io (●MN{dq} n) (●MN{dq1} n) (●MN{dq2} n) where
+    [h : IsOp d dq dq1 dq2] :
+    IsOp d (●MN{dq} n) (●MN{dq1} n) (●MN{dq2} n) where
   is_op := by rw [h.is_op.to_eq]; apply auth_dfrac_op
 
 @[rocq_alias mono_nat_lb_max_is_op]
 instance {n n1 n2 : MaxNat}
-    [h : IsOp io n n1 n2] :
-    IsOp io (◯MN n : MonoNat) (◯MN n1) (◯MN n2) where
+    [h : IsOp d n n1 n2] :
+    IsOp d (◯MN n : MonoNat) (◯MN n1) (◯MN n2) where
   is_op := by rw [h.is_op.to_eq]; exact .rfl
 
 end MonoNat
