Iris/Iris/Algebra/View.lean
@@ -333,8 +333,8 @@ theorem auth_op_auth_eqv : (●V{dq1 • dq2} a : View R) ≡ (●V{dq1} a) • 
 
 @[rocq_alias view_auth_dfrac_is_op]
 instance isOp_view_auth_dfrac {dq dq1 dq2 : DFrac} {a : A}
-    [h : IsOp io dq dq1 dq2] :
-    IsOp io (●V{dq} a : View R) (●V{dq1} a) (●V{dq2} a) where
+    [h : IsOp d dq dq1 dq2] :
+    IsOp d (●V{dq} a : View R) (●V{dq1} a) (●V{dq2} a) where
   is_op := by
     rw [h.is_op.to_eq]
     apply auth_op_auth_eqv
@@ -377,8 +377,8 @@ instance [CMRA.CoreId b] : CMRA.CoreId ((●V{.discard} a : View R) • ◯V b) 
     refine UCMRA.unit_left_id.symm
 
 @[rocq_alias view_frag_is_op]
-instance {b b1 b2 : B} [h : IsOp io b b1 b2] :
-    IsOp io (◯V b : View R) (◯V b1) (◯V b2) where
+instance {b b1 b2 : B} [h : IsOp d b b1 b2] :
+    IsOp d (◯V b : View R) (◯V b1) (◯V b2) where
   is_op := NonExpansive.eqv h.is_op
 
 @[rocq_alias view_auth_dfrac_op_invN]
